Add ChaseDerivationSkeleton and CyclicityDeriv.

ExistentialRules/ChaseSequence/ChaseDerivation.lean
@@ -1,23 +1,20 @@
 import BasicLeanDatastructures.Nat
-import PossiblyInfiniteTrees.PossiblyInfiniteList.PossiblyInfiniteList
 
 import ExistentialRules.Models.Basic
-import ExistentialRules.ChaseSequence.ChaseNode
+import ExistentialRules.ChaseSequence.ChaseDerivationSkeleton
 
 /-!
 # Chase Derivation
 
-It is time to define the chase.
-We are going to introduce slightly different representations and the `ChaseDerivation` is arguably the most basic but also most versatile one.
+Now we go from a `ChaseDerivationSkeleton` to a `ChaseDerivation`.
 
-As briefly discussed for the `ChaseNode` already,
-the chase starts on an initial fact set and then applies triggers until all triggers are obsolete, which might only be the case after infinitely many steps.
+The chase starts on an initial fact set and then applies triggers until all triggers are obsolete, which might only be the case after infinitely many steps.
 This whole process needs to be "fair", i.e. a trigger that is `active` needs to be not active after finitely many steps. This can happen by applying the trigger itself or another trigger that will make the former obsolete.
 
 We should note that chase derivations usually start on a `Database`, i.e. a finite fact set where all terms are constants.
 This is what we demand for a `ChaseBranch` later but for now it is more convenient for us to relax this condition since it is not relevant for
 most basic definitions and results.
-What we gain by relaxing the condition is that we can drop an abitrary number of `ChaseNode`s from the beginning of a derivation and still be left with a derivation. This gives the `ChaseDerivation` a more coinductive behavior that conveniently alignes with the `PossiblyInfiniteList` that is used to provide the basic structure of the derivation.
+What we gain by relaxing the condition is that we can drop an abitrary number of `ChaseNode`s from the beginning of a derivation and still be left with a derivation. This gives the `ChaseDerivation` a more coinductive behavior that conveniently alignes with the `PossiblyInfiniteList` that is used to provide the basic structure of the derivation skeleton.
 
 The goal of the chase is to eventually build a most general (i.e. universal) model of a given `KnowledgeBase` by iteratively satisfying all triggers and thereby all rules.
 For the more generic `ChaseDerivation`, we cannot quite expect this as a result but we can already show that the `ChaseDerivation.result` models all of the rules in `ChaseDerivation.result_models_rules`.
@@ -25,50 +22,21 @@ For the more generic `ChaseDerivation`, we cannot quite expect this as a result 
 
 variable {sig : Signature} [DecidableEq sig.P] [DecidableEq sig.C] [DecidableEq sig.V]
 
-section ChaseStep
-
-/-!
-## Chase Step
-
-To define how one chase step follows from the previous, we introduce two auxiliary definitions that capture two cases that can occur for a given `ChaseNode` in a `ChaseDerivation`.
-
-1. Case: There still exists an `active` trigger, in which case the next `ChaseNode` shall be defined accordingly. That is, we add the facts introduced by the trigger to the facts from the previous step and we set the origin of the `ChaseNode` to the trigger.
-
-2. Case: There is no active trigger. Then the next chase step must be undefined (`none`), i.e. the `ChaseDerivation` stops at this point.
--/
-
-def exists_trigger_opt_fs (obs : ObsoletenessCondition sig) (rules : RuleSet sig) (before : ChaseNode obs rules) (after : Option (ChaseNode obs rules)) : Prop :=
-  ∃ trg : (RTrigger (obs : LaxObsoletenessCondition sig) rules), trg.val.active before.facts ∧ ∃ i, after = some {
-    facts := before.facts ∪ (trg.val.mapped_head[i.val]'(i.isLt)).toSet,
-    origin := some ⟨trg, i⟩
-    facts_contain_origin_result := by intro _ eq; rw [Option.mem_def, Option.some_inj] at eq; rw [← eq]; apply Set.subset_union_of_subset_right; apply Set.subset_refl
-  }
-
-def not_exists_trigger_opt_fs (obs : ObsoletenessCondition sig) (rules : RuleSet sig) (before : ChaseNode obs rules) (after : Option (ChaseNode obs rules)) : Prop :=
-  ¬(∃ trg : (RTrigger obs rules), trg.val.active before.facts) ∧ after = none
-
-end ChaseStep
-
 /-!
 ## The ChaseDerivation Structure
 
-The backbone of the `ChaseDerivation` is a `PossiblyInfiniteList` of `ChaseNode`s with a couple of conditions.
+The backbone of the `ChaseDerivation` is a `ChaseDerivationSkeleton` with additional conditions.
 
-1. We enforce that there is at least an initial `ChaseNode`.
-2. At each step in the derivation, either there exists a trigger that yields the next node or there is no trigger and consequently the derivation stops at this point. This is expressed by the two auxiliary definitions above.
-3. The derivation needs to be fair. That is, for each trigger, there exists a step in the derivation from which on the trigger is not active.
+1. Each trigger used in the derivation must be active for the previous fact set.
+2. The derivation needs to be fair. That is, for each trigger, there exists a step in the derivation from which on the trigger is not active.
 
 Expressing the conditions in terms of the machinery available form the `PossiblyInfiniteList` is admittedly quite convoluted.
 As part of the framework built around the `ChaseDerivation`, we will also restate these conditions in a more accessible way. See e.g. `ChaseDerivation.fairness'`.
 -/
 
-structure ChaseDerivation (obs : ObsoletenessCondition sig) (rules : RuleSet sig) where
-  branch : PossiblyInfiniteList (ChaseNode obs rules)
-  isSome_head : branch.head.isSome
-  triggers_exist : ∀ n : Nat, ∀ before ∈ (branch.drop n).head,
-    let after := (branch.drop n).tail.head
-    (exists_trigger_opt_fs obs rules before after) ∨
-    (not_exists_trigger_opt_fs obs rules before after)
+structure ChaseDerivation (obs : ObsoletenessCondition sig) (rules : RuleSet sig) extends ChaseDerivationSkeleton obs rules where
+  triggers_active : ∀ n : Nat, ∀ before ∈ (branch.drop n).head,
+    ∀ after ∈ (branch.drop n).tail.head, ∃ orig ∈ after.origin, orig.fst.val.active before.facts
   fairness : ∀ trg : (RTrigger obs rules), ∃ i : Nat, (∃ node ∈ (branch.drop i).head, ¬ trg.val.active node.facts)
     ∧ (∀ j : Nat, ∀ node2 ∈ (branch.drop i).tail.get? j, ¬ trg.val.active node2.facts)
 
@@ -81,33 +49,34 @@ section Basics
 /-!
 ## Basic Definitions
 
-Here we introduce some auxiliary definitions and theorems and we lift some of the machinery of the underlying `PossiblyInfiniteList` to `ChaseDerivation`.
+Here we introduce some auxiliary definitions and theorems and we lift some of the machinery of the underlying `PossiblyInfiniteList` to `ChaseDerivation`. Some has already been lifted to `ChaseDerivationSkeleton`.
 -/
 
-/-- Membership of `ChaseNode`s in the `ChaseDerivation` directly corresponds to membership in the `PossiblyInfiniteList`. -/
+/-- Membership of `ChaseNode`s in the `ChaseDerivation` directly corresponds to membership in the `ChaseDerivationSkeleton`. -/
 instance : Membership (ChaseNode obs rules) (ChaseDerivation obs rules) where
-  mem cd node := node ∈ cd.branch
+  mem cd node := node ∈ cd.toChaseDerivationSkeleton
 
-/-- Each suffix of the underlying `PossiblyInfiniteList` is itself a `ChaseDerivation` as long as its head is not none. -/
-def derivation_for_branch_suffix
+/-- Each suffix of the underlying `ChaseDerivationSkeleton` is itself a `ChaseDerivation`. -/
+def derivation_for_skeleton
     (cd : ChaseDerivation obs rules)
-    (l2 : PossiblyInfiniteList (ChaseNode obs rules))
-    (suffix : l2 <:+ cd.branch)
-    (l2_head_some : l2.head.isSome) :
+    (l2 : ChaseDerivationSkeleton obs rules)
+    (suffix : l2 <:+ cd.toChaseDerivationSkeleton) :
     ChaseDerivation obs rules where
-  branch := l2
-  isSome_head := l2_head_some
-  triggers_exist := by
-    rw [PossiblyInfiniteList.IsSuffix_iff] at suffix
+  branch := l2.branch
+  isSome_head := l2.isSome_head
+  triggers_exist := l2.triggers_exist
+  triggers_active := by
+    rw [ChaseDerivationSkeleton.IsSuffix, PossiblyInfiniteList.IsSuffix_iff] at suffix
     rcases suffix with ⟨m, suffix⟩
     rw [← suffix]
     intro n
-    have := cd.triggers_exist (m + n)
+    have := cd.triggers_active (m + n)
     simp only [PossiblyInfiniteList.head_drop, PossiblyInfiniteList.get?_drop] at *
     exact this
   fairness := by
+    have l2_head_some := l2.isSome_head
     rw [Option.isSome_iff_exists] at l2_head_some; rcases l2_head_some with ⟨l2_head, l2_head_eq⟩
-    rw [PossiblyInfiniteList.IsSuffix_iff] at suffix
+    rw [ChaseDerivationSkeleton.IsSuffix, PossiblyInfiniteList.IsSuffix_iff] at suffix
     rcases suffix with ⟨m, suffix⟩
     rw [← suffix]
     intro trg
@@ -136,42 +105,22 @@ def derivation_for_branch_suffix
       simp only [← Nat.add_succ, ← Nat.add_assoc, Nat.add_sub_of_le le] at *
       exact fairness
 
-/-- The head of the `ChaseDerivation` is the initial `ChaseNode`. We know that this is never none. -/
-def head (cd : ChaseDerivation obs rules) : ChaseNode obs rules := cd.branch.head.get (cd.isSome_head)
-
-/-- The `head` is a member. -/
-theorem head_mem {cd : ChaseDerivation obs rules} : cd.head ∈ cd := by exists 0; simp [head, PossiblyInfiniteList.head_eq, PossiblyInfiniteList.get?]
-
 section Next
 
 /-!
 ### The "next" ChaseNode
 
-For a `ChaseDerivation` derivation, its `next` node is the `ChaseNode` immediately following the `head`.
-We mainly introduce a couple of theorems here that abstract away the `triggers_exist` condition from the `ChaseDerivation` definition.
+Compared to the `ChaseDerivationSkeleton` we can show some additional results for `next`.
 -/
-
-def next (cd : ChaseDerivation obs rules) : Option (ChaseNode obs rules) := cd.branch.tail.head
-
-/-- The `next` node is a member. -/
-theorem next_mem_of_mem {cd : ChaseDerivation obs rules} : ∀ next ∈ cd.next, next ∈ cd := by intro next next_mem; apply cd.branch.tail.mem_of_mem_suffix cd.branch.IsSuffix_tail; apply cd.branch.tail.head_mem; exact next_mem
-
-/-- The origin of the `next` `ChaseNode` needs to be set. -/
-theorem isSome_origin_next {cd : ChaseDerivation obs rules} {next : ChaseNode obs rules} (eq : cd.next = some next) : next.origin.isSome := by
-  have trg_ex := cd.triggers_exist 0 cd.head (by simp [PossiblyInfiniteList.drop_zero, head])
-  rw [PossiblyInfiniteList.drop_zero] at trg_ex
-  cases trg_ex with
-  | inl trg_ex => rcases trg_ex with ⟨_, _, _, trg_ex⟩; unfold ChaseDerivation.next at eq; rw [eq, Option.some_inj] at trg_ex; rw [trg_ex]; simp
-  | inr trg_ex => have contra := trg_ex.right; unfold ChaseDerivation.next at eq; simp [eq] at contra
 
 /-- The trigger used to derive `next` is active for `head`. -/
 theorem active_trigger_origin_next {cd : ChaseDerivation obs rules} {next : ChaseNode obs rules} (eq : cd.next = some next) :
     (next.origin.get (cd.isSome_origin_next eq)).fst.val.active cd.head.facts := by
-  have trg_ex := cd.triggers_exist 0 cd.head (by simp [PossiblyInfiniteList.drop_zero, head])
-  rw [PossiblyInfiniteList.drop_zero] at trg_ex
-  cases trg_ex with
-  | inl trg_ex => rcases trg_ex with ⟨trg', trg'_active, _, trg_ex⟩; unfold ChaseDerivation.next at eq; rw [eq, Option.some_inj] at trg_ex; simp only [trg_ex, Option.get_some]; exact trg'_active
-  | inr trg_ex => have contra := trg_ex.right; unfold ChaseDerivation.next at eq; simp [eq] at contra
+  have trg_act := cd.triggers_active 0 cd.head (by simp [PossiblyInfiniteList.drop_zero, ChaseDerivationSkeleton.head]) next eq
+  rcases trg_act with ⟨orig, orig_mem, trg_act⟩
+  rw [Option.mem_def] at orig_mem
+  simp only [orig_mem, Option.get_some]
+  exact trg_act
 
 /-- The `next` node is not none if and only if some trigger is active on `head`. -/
 theorem isSome_next_iff_trg_ex {cd : ChaseDerivation obs rules} : cd.next.isSome ↔ ∃ (trg : RTrigger obs rules), trg.val.active cd.head.facts := by
@@ -184,20 +133,18 @@ theorem isSome_next_iff_trg_ex {cd : ChaseDerivation obs rules} : cd.next.isSome
     apply Decidable.byContradiction
     rw [Option.not_isSome_iff_eq_none]
     intro eq_none
-    have trg_ex := cd.triggers_exist 0 cd.head (by simp [PossiblyInfiniteList.drop_zero, head])
-    rw [PossiblyInfiniteList.drop_zero] at trg_ex
-    cases trg_ex with
-    | inl trg_ex => rcases trg_ex with ⟨_, _, _, contra⟩; unfold next at eq_none; simp [eq_none] at contra
-    | inr trg_ex => apply trg_ex.left; exists trg
-
-/-- The fact set of the `next` `ChaseNode` consists exactly of the facts from `head` and the result of the trigger that introduces `next`. -/
-theorem facts_next {cd : ChaseDerivation obs rules} {next : ChaseNode obs rules} (eq : cd.next = some next) :
-    next.facts = cd.head.facts ∪ (next.origin_result (cd.isSome_origin_next eq)).toSet := by
-  have trg_ex := cd.triggers_exist 0 cd.head (by simp [PossiblyInfiniteList.drop_zero, head])
-  rw [PossiblyInfiniteList.drop_zero] at trg_ex
-  cases trg_ex with
-  | inl trg_ex => rcases trg_ex with ⟨trg', trg'_active, _, trg_ex⟩; unfold ChaseDerivation.next at eq; rw [eq, Option.some_inj] at trg_ex; simp only [trg_ex]; rfl
-  | inr trg_ex => have contra := trg_ex.right; unfold ChaseDerivation.next at eq; simp [eq] at contra
+    have fair := cd.fairness trg
+    rcases cd.fairness trg with ⟨i, ⟨node, node_mem, not_active⟩, fair⟩
+    cases i with
+    | zero =>
+      apply not_active
+      have eq : cd.head = node := by simp only [ChaseDerivationSkeleton.head]; simp only [PossiblyInfiniteList.drop_zero, Option.mem_def] at node_mem; simp [node_mem]
+      rw [← eq]
+      exact active
+    | succ i =>
+      simp only [ChaseDerivationSkeleton.next, ← PossiblyInfiniteList.empty_iff_head_none] at eq_none
+      rw [PossiblyInfiniteList.head_drop, ← PossiblyInfiniteList.get?_tail, eq_none, PossiblyInfiniteList.get?_empty] at node_mem
+      simp at node_mem
 
 end Next
 
@@ -206,40 +153,33 @@ section Suffixes
 /-!
 ### ChaseDerivation Suffixes
 
-We define a suffix relation on `ChaseDerivation` simply as the suffix relation of the underlying `PossiblyInfiniteList`.
-We also use this to state the fairness condition more nicely.
+Suffixes on `ChaseDerivation`s allow us to state the fairness condition more nicely.
 -/
 
-def IsSuffix (cd1 cd2 : ChaseDerivation obs rules) : Prop := cd1.branch <:+ cd2.branch
+def IsSuffix (cd1 cd2 : ChaseDerivation obs rules) : Prop := ChaseDerivationSkeleton.IsSuffix cd1.toChaseDerivationSkeleton cd2.toChaseDerivationSkeleton
 infixl:50 " <:+ " => IsSuffix
 
 /-- Members of our suffix are also our members. -/
-theorem mem_of_mem_suffix {cd1 cd2 : ChaseDerivation obs rules} (suffix : cd1 <:+ cd2) : ∀ node ∈ cd1, node ∈ cd2 := by
-  rintro node ⟨n, node_eq⟩
-  rcases suffix with ⟨m, suffix⟩
-  exists m + n
-  rw [← suffix, InfiniteList.get_drop] at node_eq
-  exact node_eq
+theorem mem_of_mem_suffix {cd1 cd2 : ChaseDerivation obs rules} (suffix : cd1 <:+ cd2) : ∀ node ∈ cd1, node ∈ cd2 := ChaseDerivationSkeleton.mem_of_mem_suffix suffix
 
 /-- Each `ChaseNode` in the `ChaseDerivation` induces a subderivation. -/
 theorem subderivation_of_node_mem {cd : ChaseDerivation obs rules} {node : ChaseNode obs rules} (node_mem : node ∈ cd) :
     ∃ (cd2 : ChaseDerivation obs rules), cd2.head = node ∧ cd2 <:+ cd := by
-  rcases node_mem with ⟨n, node_mem⟩
-  exists cd.derivation_for_branch_suffix (cd.branch.drop n) (cd.branch.IsSuffix_drop n) (by simp only [PossiblyInfiniteList.head_drop, PossiblyInfiniteList.get?, node_mem]; simp)
-  constructor
-  . simp only [derivation_for_branch_suffix, head, PossiblyInfiniteList.head_drop, PossiblyInfiniteList.get?, node_mem, Option.get_some]
-  . exact cd.branch.IsSuffix_drop n
+  rcases cd.toChaseDerivationSkeleton.subderivation_of_node_mem node_mem with ⟨cds2, head_eq, suffix⟩
+  exists cd.derivation_for_skeleton cds2 suffix
 
 /-- Fairness can be stated as: For each trigger, there exists a subderivation such that the trigger is not active for all nodes in the subderivation. -/
 theorem fairness' {cd : ChaseDerivation obs rules} : ∀ (trg : RTrigger obs rules), ∃ (cd2 : ChaseDerivation obs rules), cd2 <:+ cd ∧ ∀ node ∈ cd2, ¬ trg.val.active node.facts := by
   intro trg
   rcases cd.fairness trg with ⟨n, ⟨node, node_mem, fairness_head⟩, fairness_tail⟩
-  exists cd.derivation_for_branch_suffix (cd.branch.drop n) (cd.branch.IsSuffix_drop n) (by rw [node_mem]; simp)
+  let cds2 := cd.derivation_for_branch_suffix (cd.branch.drop n) (cd.branch.IsSuffix_drop n) (by rw [node_mem]; simp)
+  let cd2 := cd.derivation_for_skeleton cds2 (cd.branch.IsSuffix_drop n)
+  exists cd2
   constructor
   . exact cd.branch.IsSuffix_drop n
   . intro node2 node2_mem
     rcases node2_mem with ⟨m, node2_mem⟩
-    simp only [derivation_for_branch_suffix, PossiblyInfiniteList.drop, InfiniteList.get_drop] at node2_mem
+    simp only [cd2, derivation_for_skeleton, cds2, ChaseDerivationSkeleton.derivation_for_branch_suffix, PossiblyInfiniteList.drop, InfiniteList.get_drop] at node2_mem
     cases m with
     | zero => simp only [PossiblyInfiniteList.head_drop, PossiblyInfiniteList.get?] at node_mem; rw [Nat.add_zero, node_mem, Option.some_inj] at node2_mem; rw [← node2_mem]; exact fairness_head
     | succ m =>
@@ -255,83 +195,29 @@ section Tail
 
 /-!
 ### Tail
-
-If `next` exists, we can drop the first element from the `ChaseDerivation` and obtain a new `ChaseDerivation`, which, inspired by the `PossiblyInfiniteList`, we call the `tail`.
 -/
 
 def tail (cd : ChaseDerivation obs rules) (next_some : cd.next.isSome) : ChaseDerivation obs rules :=
-  cd.derivation_for_branch_suffix cd.branch.tail (cd.branch.IsSuffix_tail) next_some
+  cd.derivation_for_skeleton (ChaseDerivationSkeleton.tail cd.toChaseDerivationSkeleton next_some) (cd.branch.IsSuffix_tail)
 
 /-- The `head` of the `tail` is `next`. -/
-theorem head_tail {cd : ChaseDerivation obs rules} {next_some : cd.next.isSome} : some (cd.tail next_some).head = cd.next := by
-  unfold tail head ChaseDerivation.next derivation_for_branch_suffix
-  simp only [Option.some_get]
+theorem head_tail {cd : ChaseDerivation obs rules} {next_some : cd.next.isSome} : some (cd.tail next_some).head = cd.next := ChaseDerivationSkeleton.head_tail
 
 /-- The `head` of the `tail` is `next`. -/
-theorem head_tail' {cd : ChaseDerivation obs rules} {next_some : cd.next.isSome} : (cd.tail next_some).head = cd.next.get next_some := by rfl
+theorem head_tail' {cd : ChaseDerivation obs rules} {next_some : cd.next.isSome} : (cd.tail next_some).head = cd.next.get next_some := ChaseDerivationSkeleton.head_tail'
 
 /-- `next` is a member of the `tail`. -/
-theorem next_mem_tail {cd : ChaseDerivation obs rules} {next_some : cd.next.isSome} : ∀ next ∈ cd.next, next ∈ cd.tail next_some := by
-  intro next next_mem
-  have : next = cd.next.get next_some := by
-    conv => right; left; rw [next_mem]
-    simp
-  rw [this, ← head_tail']
-  exact head_mem
+theorem next_mem_tail {cd : ChaseDerivation obs rules} {next_some : cd.next.isSome} : ∀ next ∈ cd.next, next ∈ cd.tail next_some := ChaseDerivationSkeleton.next_mem_tail
 
 /-- A node is a member if and only if it is either the head or it is a member of the tail. -/
-theorem mem_iff_eq_head_or_mem_tail {cd : ChaseDerivation obs rules} {node : ChaseNode obs rules} : node ∈ cd ↔ node = cd.head ∨ ∃ h, node ∈ cd.tail h := by
-  constructor
-  . rintro ⟨n, mem⟩
-    cases n with
-    | zero => apply Or.inl; simp [head, PossiblyInfiniteList.head, InfiniteList.head, mem]
-    | succ n =>
-      apply Or.inr;
-      exists (by
-        rw [Option.isSome_iff_ne_none]; intro contra; simp only [next, PossiblyInfiniteList.head_eq, PossiblyInfiniteList.get?_tail] at contra
-        have := cd.branch.get?_eq_none_of_le_of_eq_none contra n.succ (by simp)
-        simp only [PossiblyInfiniteList.get?] at this; rw [this] at mem
-        simp at mem)
-      exists n
-  . intro or; cases or with
-    | inl eq_head => rw [eq_head]; exact cd.head_mem
-    | inr mem_tail => rcases mem_tail with ⟨_, mem_tail⟩; apply mem_of_mem_suffix _ _ mem_tail; exact cd.branch.IsSuffix_tail
+theorem mem_iff_eq_head_or_mem_tail {cd : ChaseDerivation obs rules} {node : ChaseNode obs rules} : node ∈ cd ↔ node = cd.head ∨ ∃ h, node ∈ cd.tail h := ChaseDerivationSkeleton.mem_iff_eq_head_or_mem_tail
 
 /-- A derivation is a suffix of another if and only if both are the same or the first is a suffix of the second's tail. -/
 theorem suffix_iff_eq_or_suffix_tail {cd1 cd2 : ChaseDerivation obs rules} : cd1 <:+ cd2 ↔ cd1 = cd2 ∨ ∃ h, cd1 <:+ cd2.tail h := by
-  -- TODO: maybe we should extract a result like this to InfiniteList directly
-  constructor
-  . rintro ⟨n, suffix⟩
-    cases n with
-    | zero => apply Or.inl; rw [InfiniteList.drop_zero] at suffix; apply Eq.symm; rw [ChaseDerivation.mk.injEq, PossiblyInfiniteList.mk.injEq]; exact suffix
-    | succ n =>
-      apply Or.inr
-      exists (by
-        rw [Option.isSome_iff_ne_none]
-        intro contra
-        have := cd2.branch.get?_eq_none_of_le_of_eq_none contra (n+1) (by simp)
-        simp only [PossiblyInfiniteList.get?] at this
-        rw [InfiniteList.ext_iff] at suffix
-        specialize suffix 0
-        rw [InfiniteList.get_drop, Nat.add_zero, this] at suffix
-        have contra := cd1.isSome_head
-        rw [Option.isSome_iff_ne_none] at contra
-        apply contra
-        simp only [PossiblyInfiniteList.head_eq, PossiblyInfiniteList.get?]
-        rw [← suffix])
-      exists n
-      simp only [tail, derivation_for_branch_suffix, PossiblyInfiniteList.tail]
-      apply InfiniteList.ext
-      intro m
-      simp only [InfiniteList.get_tail, InfiniteList.get_drop]
-      rw [InfiniteList.ext_iff] at suffix
-      simp only [InfiniteList.get_drop] at suffix
-      have : (n+m).succ = (n + 1 + m) := by omega
-      rw [this]
-      apply suffix m
-  . intro h; cases h with
-    | inl eq => rw [eq]; exact PossiblyInfiniteList.IsSuffix_refl
-    | inr suffix => rcases suffix with ⟨h, suffix⟩; apply PossiblyInfiniteList.IsSuffix_trans suffix; exact PossiblyInfiniteList.IsSuffix_tail
+  simp only [IsSuffix]
+  rw [ChaseDerivationSkeleton.suffix_iff_eq_or_suffix_tail]
+  rw [ChaseDerivation.mk.injEq]
+  rfl
 
 end Tail
 
@@ -340,9 +226,7 @@ section InductionPrinciple
 /-!
 ### Induction Principle for Members
 
-Similar to `PossiblyInfiniteList.mem_rec`, we define an induction principle to show
-properties of `ChaseNode`s in a `ChaseDerivation`.
-For this, we introduce `ChaseDerivatio.Node` as the subtype of `ChaseNode` that features a membership proof.
+We lift `ChaseDerivationSkeleton.mem_rec` to `ChaseDerivation`.
 -/
 
 abbrev Node (cd : ChaseDerivation obs rules) := { node : ChaseNode obs rules // node ∈ cd}
@@ -358,47 +242,20 @@ theorem mem_rec
     (step : ∀ (cd2 : ChaseDerivation obs rules), (suffix : cd2 <:+ cd) -> motive ⟨cd2.head, mem_of_mem_suffix suffix _ cd2.head_mem⟩ -> ∀ next, (next_mem : next ∈ cd2.next) -> motive ⟨next, mem_of_mem_suffix suffix _ (cd2.next_mem_of_mem _ next_mem)⟩)
     (node : Node cd) :
     motive node := by
-  induction node using PossiblyInfiniteList.mem_rec with
-  | head head' mem => unfold ChaseDerivation.head at head; rw [Option.mem_def] at mem; simp only [mem, Option.get_some] at head; exact head
-  | step l2 suffix ih next next_mem =>
-    rcases ih with ⟨head, head_mem, ih⟩
-    let cd2 : ChaseDerivation obs rules := cd.derivation_for_branch_suffix l2 suffix (by rw [head_mem]; simp)
-    apply step cd2 suffix
-    . simp only [cd2, derivation_for_branch_suffix, ChaseDerivation.head];
-      conv => right; left; left; rw [head_mem]
-      simp only [Option.get_some]
-      exact ih
-    . exact next_mem
+  induction node using ChaseDerivationSkeleton.mem_rec with
+  | head => exact head
+  | step cds2 suffix ih next next_mem =>
+    let cd2 := cd.derivation_for_skeleton cds2 suffix
+    exact step cd2 suffix ih _ next_mem
 
-/-- A node is a member of the `tail` if and only if there is a subderivation where the node is in the `next` position. Part of this proof uses the induction principle defined above. -/
+/-- A node is a member of the `tail` if and only if there is a subderivation where the node is in the `next` position. -/
 theorem mem_tail_iff {cd : ChaseDerivation obs rules} {next_some : cd.next.isSome} {node : ChaseNode obs rules} :
     node ∈ cd.tail next_some ↔ ∃ cd2, cd2 <:+ cd ∧ cd2.next = some node := by
+  have : node ∈ cd.tail next_some ↔ node ∈ cd.toChaseDerivationSkeleton.tail next_some := by rfl
+  rw [this, ChaseDerivationSkeleton.mem_tail_iff]
   constructor
-  . intro node_mem
-    let node' : (cd.tail next_some).Node := ⟨node, node_mem⟩
-    show ∃ cd2, cd2 <:+ cd ∧ cd2.next = some node'.val
-    induction node' using mem_rec with
-    | head => exists cd; constructor; exact cd.branch.IsSuffix_refl; rw [head_tail]
-    | step cd3 suffix ih next next_mem =>
-      exists cd3; constructor
-      . apply cd3.branch.IsSuffix_trans suffix; exact cd.branch.IsSuffix_tail
-      . exact next_mem
-  . rintro ⟨cd2, suffix, next_eq⟩
-    have : cd2.tail (by simp [next_eq]) <:+ cd.tail next_some := by
-      -- TODO: maybe we should extract a result like this to InfiniteList directly
-      rcases suffix with ⟨n, suffix⟩
-      exists n
-      simp only [tail, derivation_for_branch_suffix, PossiblyInfiniteList.tail]
-      apply InfiniteList.ext
-      intro m
-      simp only [InfiniteList.get_tail, InfiniteList.get_drop]
-      rw [InfiniteList.ext_iff] at suffix
-      simp only [InfiniteList.get_drop] at suffix
-      apply suffix m.succ
-    apply mem_of_mem_suffix this
-    rw [← head_tail (next_some := by simp [next_eq]), Option.some_inj] at next_eq
-    simp only [← next_eq]
-    apply head_mem
+  . rintro ⟨cds2, suf, next_mem⟩; exists cd.derivation_for_skeleton cds2 suf
+  . rintro ⟨cd2, suf, next_mem⟩; exists cd2.toChaseDerivationSkeleton
 
 end InductionPrinciple
 
@@ -409,30 +266,15 @@ section FactMonotonicity
 /-!
 ## Subset Monotonicity of Facts in ChaseNodes
 
-Since `ChaseNodes` always extend the previous facts, the fact sets can only be growing along the `ChaseDerivation`.
-This has a couple of convenient implications. For example, we can never see the same `ChaseNode` twice as otherwise the trigger in second occurrence would already be obsolete.
+Compared to `ChaseDerivationSkeleton`, we get a couple of nice implications out of the subset monotonicity of fact sets. For example, we can never see the same `ChaseNode` twice as otherwise the trigger in second occurrence would already be obsolete.
 -/
 
 /-- Each member's facts contain the head facts. Note that this extends to arbitrary pairs of members since each member always induces a subderivation where it acts as the head. -/
-theorem facts_node_subset_every_mem {cd : ChaseDerivation obs rules} : ∀ node ∈ cd, cd.head.facts ⊆ node.facts := by
-  intro node node_mem
-  let node' : cd.Node := ⟨node, node_mem⟩
-  show cd.head.facts ⊆ node'.val.facts
-  induction node' using mem_rec with
-  | head => apply Set.subset_refl
-  | step cd2 suffix subset next next_eq =>
-    apply Set.subset_trans subset
-    rw [cd2.facts_next next_eq]
-    apply Set.subset_union_of_subset_left
-    apply Set.subset_refl
+theorem facts_node_subset_every_mem {cd : ChaseDerivation obs rules} : ∀ node ∈ cd, cd.head.facts ⊆ node.facts :=
+  ChaseDerivationSkeleton.facts_node_subset_every_mem
 
 /-- A first implication of `facts_node_subset_every_mem` is that, considering one of our subderivations, each of our members either has all of its facts contained in the head of the subderivation or it is itself a member of the subderivation. -/
-theorem mem_suffix_of_mem {cd1 cd2 : ChaseDerivation obs rules} (suffix : cd1 <:+ cd2) : ∀ node ∈ cd2, node.facts ⊆ cd1.head.facts ∨ node ∈ cd1 := by
-  intro node node_mem
-  rcases subderivation_of_node_mem node_mem with ⟨cd3, cd3_head, suffix'⟩
-  cases PossiblyInfiniteList.suffix_or_suffix_of_suffix suffix suffix' with
-  | inl suffix => apply Or.inl; rw [← cd3_head]; apply cd3.facts_node_subset_every_mem; apply mem_of_mem_suffix suffix; apply cd1.head_mem
-  | inr suffix => apply Or.inr; rw [← cd3_head]; apply mem_of_mem_suffix suffix; apply cd3.head_mem
+theorem mem_suffix_of_mem {cd1 cd2 : ChaseDerivation obs rules} (suffix : cd1 <:+ cd2) : ∀ node ∈ cd2, node.facts ⊆ cd1.head.facts ∨ node ∈ cd1 := ChaseDerivationSkeleton.mem_suffix_of_mem suffix
 
 /-- The `head` cannot occur in the `tail`. Otherwise, it would be introduced using a trigger but then this trigger is already obsolete since all the facts from `head` already occur in the very beginning. We use `ObsoletenessCondition.contains_trg_result_implies_cond` here. -/
 theorem head_not_mem_tail {cd : ChaseDerivation obs rules} : ∀ h, ¬ cd.head ∈ cd.tail h := by
@@ -468,28 +310,19 @@ section Predecessors
 ## Predecessor Relation
 
 Since we learned that `ChaseNode`s cannot occur multiple times in the same `ChaseDerivation`,
-we can define predecessor relation (`≼`), which is a total order on `ChaseDerivation.Node`.
+the predecessor relation defined on `ChaseDerivationSkeleton` is now a total order on `ChaseDerivation.Node`.
 This is particularly nice, since we can do this while completely ignoring indices of the nodes in the underlying `PossiblyInfiniteList`.
 -/
 
-/-- A node $n$ is a predecessor of a node $m$ if there is a subderivation there $n$ is the head and $m$ is an arbitrary member. -/
-def predecessor {cd : ChaseDerivation obs rules} (n1 n2 : Node cd) : Prop := ∃ cd2, cd2 <:+ cd ∧ cd2.head = n1.val ∧ n2.val ∈ cd2
-infixl:50 " ≼ " => predecessor
-
-/-- The predecessor relation is stable across suffixes. That is, predecessor in our suffix are also predecessor for us. We only need to cast the nodes. -/
-theorem predecessor_of_suffix {cd cd2 : ChaseDerivation obs rules} {n1 n2 : Node cd} (suffix : cd <:+ cd2) : n1 ≼ n2 -> (n1.cast_suffix suffix) ≼ (n2.cast_suffix suffix) := by
-  rintro ⟨cd3, suffix', head_eq, mem⟩
-  exists cd3; constructor
-  . exact cd3.branch.IsSuffix_trans suffix' suffix
+/-- We could also define the predecessor relation directly on `ChaseDerivation`s. This theorem shows how this would look. -/
+theorem predecessor_iff {cd : ChaseDerivation obs rules} (n1 n2 : Node cd) : n1 ≼ n2 ↔ ∃ cd2, cd2 <:+ cd ∧ cd2.head = n1.val ∧ n2.val ∈ cd2 := by
   constructor
-  . rw [head_eq]; rfl
-  . exact mem
-
-/-- The predecessor relation is reflexive. -/
-theorem predecessor_refl {cd : ChaseDerivation obs rules} {node : Node cd} : node ≼ node := by rcases cd.subderivation_of_node_mem node.property with ⟨cd2, head_eq, suffix⟩; exists cd2; simp only [suffix, head_eq, true_and]; rw [← head_eq]; exact cd2.head_mem
+  . rintro ⟨cds2, suf, head, mem⟩; exists cd.derivation_for_skeleton cds2 suf
+  . rintro ⟨cd2, suf, head, mem⟩; exists cd2.toChaseDerivationSkeleton
 
 /-- The predecessor relation is antisymmetric. -/
 theorem predecessor_antisymm {cd : ChaseDerivation obs rules} {n1 n2 : Node cd} : n1 ≼ n2 -> n2 ≼ n1 -> n1 = n2 := by
+  rw [predecessor_iff, predecessor_iff]
   rintro ⟨cd1, suffix1, head_eq1, prec1⟩ ⟨cd2, suffix2, head_eq2, prec2⟩
   have : cd1 = cd2 := by
     apply eq_of_suffix_of_head_mem _ (by rw [head_eq2]; exact prec1)
@@ -500,30 +333,12 @@ theorem predecessor_antisymm {cd : ChaseDerivation obs rules} {n1 n2 : Node cd} 
 
 /-- The predecessor relation is transitive. -/
 theorem predecessor_trans {cd : ChaseDerivation obs rules} {n1 n2 n3 : Node cd} : n1 ≼ n2 -> n2 ≼ n3 -> n1 ≼ n3 := by
+  rw [predecessor_iff, predecessor_iff, predecessor_iff]
   rintro ⟨cd1, suffix1, head_eq1, prec1⟩ ⟨cd2, suffix2, head_eq2, prec2⟩
   exists cd1; simp only [suffix1, head_eq1, true_and]
   apply mem_of_mem_suffix _ _ prec2
   apply suffix_of_suffix_of_suffix_of_head_mem suffix1 suffix2
   rw [head_eq2]; exact prec1
-
-/-- The predecessor relation is total. -/
-theorem predecessor_total {cd : ChaseDerivation obs rules} (n1 n2 : Node cd) : n1 ≼ n2 ∨ n2 ≼ n1 := by
-  rcases cd.subderivation_of_node_mem n1.property with ⟨cd1, head1, suf1⟩
-  rcases cd.subderivation_of_node_mem n2.property with ⟨cd2, head2, suf2⟩
-  cases PossiblyInfiniteList.suffix_or_suffix_of_suffix suf1 suf2 with
-  | inl suffix => apply Or.inr; exists cd2; simp only [suf2, head2, true_and]; apply cd1.mem_of_mem_suffix; exact suffix; rw [← head1]; exact cd1.head_mem
-  | inr suffix => apply Or.inl; exists cd1; simp only [suf1, head1, true_and]; apply cd2.mem_of_mem_suffix; exact suffix; rw [← head2]; exact cd2.head_mem
-
-/-- The `head` is a predecessor of `next`. -/
-theorem head_prec_next {cd : ChaseDerivation obs rules} : ∀ {next}, (mem : next ∈ cd.next) -> ⟨cd.head, cd.head_mem⟩ ≼ ⟨next, cd.next_mem_of_mem _ mem⟩ := by
-  intro next next_mem; exact ⟨cd, cd.branch.IsSuffix_refl, rfl, cd.next_mem_of_mem _ next_mem⟩
-
-/-- The facts of our predecessor are a subset of our facts. -/
-theorem facts_node_subset_of_prec {cd : ChaseDerivation obs rules} {node1 node2 : cd.Node} : node1 ≼ node2 -> node1.val.facts ⊆ node2.val.facts := by
-  rintro ⟨cd2, suffix, head_eq, mem⟩
-  rw [← head_eq]
-  apply facts_node_subset_every_mem
-  exact mem
 
 /-- We can express fairness in terms of the predecessor relation: For each trigger, there is a node such that the trigger is not active for each of the node's successors. -/
 theorem fairness_prec {cd : ChaseDerivation obs rules} : ∀ (trg : RTrigger obs rules), ∃ (node : cd.Node), ∀ node2, node ≼ node2 -> ¬ trg.val.active node2.val.facts := by
@@ -532,6 +347,7 @@ theorem fairness_prec {cd : ChaseDerivation obs rules} : ∀ (trg : RTrigger obs
   exists ⟨cd2.head, cd2.mem_of_mem_suffix suffix _ cd2.head_mem⟩
   intro node2 prec
   apply fair
+  rw [predecessor_iff] at prec
   rcases prec with ⟨cd3, suf3, head3, node2_mem_cd3⟩
   simp only at head3
   have : cd3 = cd2 := by
@@ -541,27 +357,11 @@ theorem fairness_prec {cd : ChaseDerivation obs rules} : ∀ (trg : RTrigger obs
   rw [← this]
   exact node2_mem_cd3
 
-
 section StrictPredecessor
 
 /-!
-We also define a strict version of the predecessor relation (`≺`) in the obvious way.
-By that, we obtain a strict total order on `ChaseDerivation.Node`.
+The strict version of the predecessor is a strict total order on `ChaseDerivation.Node` for the `ChaseDerivation`.
 -/
-
-/-- A node is a strict predecessor of another if it is a predecessor but not equal. -/
-def strict_predecessor {cd : ChaseDerivation obs rules} (n1 n2 : Node cd) : Prop := n1 ≼ n2 ∧ n1 ≠ n2
-infixl:50 " ≺ " => strict_predecessor
-
-/-- As for the predecessor relation, we can show that the relation is stable across suffixes given that we cast the nodes. -/
-theorem strict_predecessor_of_suffix {cd cd2 : ChaseDerivation obs rules} {n1 n2 : Node cd} (suffix : cd <:+ cd2) : n1 ≺ n2 -> (n1.cast_suffix suffix) ≺ (n2.cast_suffix suffix) := by
-  intro prec
-  constructor
-  . apply predecessor_of_suffix suffix; exact prec.left
-  . simp only [Node.cast_suffix]; intro contra; rw [Subtype.mk.injEq] at contra; apply prec.right; rw [Subtype.mk.injEq]; exact contra
-
-/-- The strict predecessor relation is irreflexive. -/
-theorem strict_predecessor_irreflexive {cd : ChaseDerivation obs rules} {n : Node cd} : ¬ n ≺ n := by intro contra; apply contra.right; rfl
 
 /-- The strict predecessor relation is asymmetric. -/
 theorem strict_predecessor_asymmetric {cd : ChaseDerivation obs rules} {n1 n2 : Node cd} : n1 ≺ n2 -> ¬ n2 ≺ n1 := by
@@ -577,13 +377,6 @@ theorem strict_predecessor_trans {cd : ChaseDerivation obs rules} {n1 n2 n3 : No
     rw [contra]
     exact prec2
 
-/-- The strict predecessor relation is total. -/
-theorem strict_predecessor_total {cd : ChaseDerivation obs rules} {n1 n2 : Node cd} : n1 ≠ n2 -> n1 ≺ n2 ∨ n2 ≺ n1 := by
-  intro ne
-  cases predecessor_total n1 n2 with
-  | inl prec => apply Or.inl; constructor; exact prec; exact ne
-  | inr prec => apply Or.inr; constructor; exact prec; exact Ne.symm ne
-
 /-- The `head` is a strict predecessor of `next`. -/
 theorem head_strict_prec_next {cd : ChaseDerivation obs rules} : ∀ {next}, (mem : next ∈ cd.next) -> ⟨cd.head, cd.head_mem⟩ ≺ ⟨next, cd.next_mem_of_mem _ mem⟩ := by
   intro next next_mem
@@ -596,17 +389,10 @@ theorem head_strict_prec_next {cd : ChaseDerivation obs rules} : ∀ {next}, (me
     apply cd.next_mem_tail
     exact next_mem
 
-/-- A predecessor is either equal or a strict predecessor. -/
-theorem eq_or_strict_of_predecessor {cd : ChaseDerivation obs rules} {n1 n2 : Node cd} : n1 ≼ n2 -> n1 = n2 ∨ n1 ≺ n2 := by
-  intro prec
-  cases Classical.em (n1 = n2) with
-  | inl eq => apply Or.inl; exact eq
-  | inr ne => apply Or.inr; exact ⟨prec, ne⟩
-
 /-- The facts of a strict successor cannot be a subset of our facts. This is because strict successor nodes can only be introduced by active triggers. But if a trigger only produces facts that already exist, then it cannot be active. -/
 theorem facts_not_subset_of_strict_predecessor {cd : ChaseDerivation obs rules} {n1 n2 : Node cd} : n1 ≺ n2 -> ¬ n2.val.facts ⊆ n1.val.facts := by
   intro prec contra
-  rcases prec.left with ⟨d, suf, head, mem⟩
+  rcases (predecessor_iff _ _).mp prec.left with ⟨d, suf, head, mem⟩
   rcases cd.subderivation_of_node_mem n2.property with ⟨d2, head2, suf2⟩
   have suf3 : d2 <:+ d := suffix_of_suffix_of_suffix_of_head_mem suf suf2 (by rw [head2]; exact mem)
   cases ChaseDerivation.suffix_iff_eq_or_suffix_tail.mp suf3 with
@@ -619,6 +405,7 @@ theorem facts_not_subset_of_strict_predecessor {cd : ChaseDerivation obs rules} 
     apply ObsoletenessCondition.contains_trg_result_implies_cond
     have : next.facts ⊆ d.head.facts := by
       have : ⟨next, d.next_mem_of_mem _ next_some⟩ ≼ ⟨n2.val, by apply ChaseDerivation.mem_of_mem_suffix (d2.branch.IsSuffix_trans suf3 d.branch.IsSuffix_tail); rw [← head2]; exact d2.head_mem⟩ := by
+        rw [predecessor_iff]
         exists d.tail (by simp [next_some])
         constructor
         . exact PossiblyInfiniteList.IsSuffix_tail
@@ -639,64 +426,8 @@ section ChaseResult
 /-!
 ## Chase Result
 
-Here, we define the result of a `ChaseDerivation`, which is simply the `FactSet` that is the union of all facts of all `ChaseNode`s.
+Compared to the `ChaseDerivationSkeleton`, the result is now a model for all rules.
 -/
-
-def result (cd : ChaseDerivation obs rules) : FactSet sig :=
-  fun f => ∃ node ∈ cd, f ∈ node.facts
-
-/-- Every node's facts occur in the result. -/
-theorem facts_node_subset_result {cd : ChaseDerivation obs rules} : ∀ node ∈ cd, node.facts ⊆ cd.result := by intro node _ _ _; exists node
-
-/-- The result of our suffix is the same our result. -/
-theorem result_suffix {cd1 cd2 : ChaseDerivation obs rules} (suffix : cd1 <:+ cd2) : cd1.result = cd2.result := by
-  apply Set.ext
-  intro f
-  constructor
-  . rintro ⟨node, node_mem, f_mem⟩; apply cd2.facts_node_subset_result; exact mem_of_mem_suffix suffix _ node_mem; exact f_mem
-  . rintro ⟨node, node_mem, f_mem⟩
-    cases mem_suffix_of_mem suffix _ node_mem with
-    | inl mem_suffix => apply cd1.facts_node_subset_result; exact cd1.head_mem; apply mem_suffix; exact f_mem
-    | inr mem_suffix => apply cd1.facts_node_subset_result; exact mem_suffix; exact f_mem
-
-/-- For each (finite) list of facts in the result, there is a node that that contains all of them. -/
-theorem facts_mem_some_node_of_mem_result {cd : ChaseDerivation obs rules} : ∀ (l : List (Fact sig)), l.toSet ⊆ cd.result -> ∃ node ∈ cd, l.toSet ⊆ node.facts := by
-  intro l
-  induction l with
-  | nil => intros; exists cd.head; constructor; exact cd.head_mem; intro _ contra; simp [List.mem_toSet] at contra
-  | cons f l ih =>
-    intro subset
-    rcases subset f (by simp [List.mem_toSet]) with ⟨node_f, node_f_mem, f_mem⟩
-    rcases ih (by intro f f_mem; apply subset; rw [List.mem_toSet] at f_mem; simp [List.mem_toSet, f_mem]) with ⟨node_ih, node_ih_mem, l_subset⟩
-    rcases cd.subderivation_of_node_mem node_f_mem with ⟨cd_f, cd_f_head, cd_f_suffix⟩
-    cases mem_suffix_of_mem cd_f_suffix _ node_ih_mem with
-    | inl mem_suffix =>
-      exists node_f
-      constructor
-      . exact node_f_mem
-      . intro e e_mem
-        rw [List.mem_toSet, List.mem_cons] at e_mem
-        cases e_mem with
-        | inl e_mem => rw [e_mem]; exact f_mem
-        | inr e_mem => rw [← cd_f_head]; apply mem_suffix; apply l_subset; rw [List.mem_toSet]; exact e_mem
-    | inr mem_suffix =>
-      exists node_ih
-      constructor
-      . exact node_ih_mem
-      . intro e e_mem
-        rw [List.mem_toSet, List.mem_cons] at e_mem
-        cases e_mem with
-        | inr e_mem => apply l_subset; rw [List.mem_toSet]; exact e_mem
-        | inl e_mem =>
-          rw [e_mem]
-          apply cd_f.facts_node_subset_every_mem _ mem_suffix
-          rw [cd_f_head]; exact f_mem
-
-/-- If a trigger is loaded for the result, then it is loaded for some node in the derivation. -/
-theorem trg_loaded_for_some_node_of_trg_loaded_for_result {cd : ChaseDerivation obs rules} : ∀ trg : Trigger obs, trg.loaded cd.result -> ∃ node ∈ cd, trg.loaded node.facts := by
-  intro trg trg_loaded
-  apply cd.facts_mem_some_node_of_mem_result
-  exact trg_loaded
 
 /-- The result is a model of all rules. This is true because otherwise, there would be an active trigger on the result. But then, this trigger needs to be active for some node and the hence it needs to become inactive at some point due to fairness. Hence it cannot be active on the result. Contradiction! -/
 theorem result_models_rules {cd : ChaseDerivation obs rules} : cd.result.modelsRules rules := by
@@ -719,7 +450,7 @@ theorem result_models_rules {cd : ChaseDerivation obs rules} : cd.result.modelsR
     apply cd_obs.head_mem
   . intro contra
     apply contra_not_obs
-    rw [← result_suffix (PossiblyInfiniteList.IsSuffix_trans cd_obs_suffix cd_loaded_suffix)]
+    rw [← ChaseDerivationSkeleton.result_suffix (PossiblyInfiniteList.IsSuffix_trans cd_obs_suffix cd_loaded_suffix)]
     apply obs.monotone
     . apply cd_obs.facts_node_subset_result; apply cd_obs.head_mem
     . exact contra
@@ -750,7 +481,7 @@ theorem constants_node_subset_constants_fs_union_constants_rules {cd : ChaseDeri
     apply Set.subset_union_of_subset_left
     apply Set.subset_refl
   | step cd2 suffix ih next next_eq =>
-    rw [facts_next next_eq]
+    rw [ChaseDerivationSkeleton.facts_next next_eq]
     intro c c_mem
     rw [FactSet.constants_union] at c_mem
     cases c_mem with
@@ -826,7 +557,7 @@ theorem functional_term_originates_from_some_trigger
         rcases ih with ⟨node2, prec, t_mem⟩
         apply Or.inr; exists node2; constructor;
         . apply predecessor_trans prec
-          exact predecessor_of_suffix suffix (head_prec_next next_mem)
+          exact ChaseDerivationSkeleton.predecessor_of_suffix suffix (ChaseDerivationSkeleton.head_prec_next next_mem)
         . exact t_mem
 
     cases t_mem with
@@ -840,7 +571,7 @@ theorem functional_term_originates_from_some_trigger
       cases t_mem with
       | inr t_mem =>
         apply Or.inr; exists ⟨next, cd2.mem_of_mem_suffix suffix _ (cd2.next_mem_of_mem _ next_mem)⟩; constructor
-        . exact predecessor_refl
+        . exact ChaseDerivationSkeleton.predecessor_refl
         . exists next.origin.get (cd2.isSome_origin_next next_mem)
           simp only [Option.get_mem, true_and]
           exact t_mem
@@ -915,30 +646,31 @@ This forces us to take into account specific node indices and therefore requires
 theorem node_has_unique_position (cd : ChaseDerivation obs rules) : ∀ node, ∀ i j, i < j -> cd.branch.get? i = some node -> cd.branch.get? j ≠ some node := by
   intro node i j lt eq_i eq_j
   have le := Nat.le_pred_of_lt lt
-  let cd2 := cd.derivation_for_branch_suffix (cd.branch.drop j.pred) (PossiblyInfiniteList.IsSuffix_drop j.pred) (by
+  let cds2 := cd.derivation_for_branch_suffix (cd.branch.drop j.pred) (PossiblyInfiniteList.IsSuffix_drop j.pred) (by
     rw [Option.isSome_iff_ne_none]; intro contra
     have := cd.branch.no_holes' j.pred contra
     rw [Nat.succ_pred (Nat.ne_zero_of_lt lt)] at this
     rw [eq_j] at this
     simp at this
   )
+  let cd2 := cd.derivation_for_skeleton cds2 (PossiblyInfiniteList.IsSuffix_drop j.pred)
   have next_eq : cd2.next = some node := by
-    simp only [next, cd2, derivation_for_branch_suffix, PossiblyInfiniteList.tail_drop, PossiblyInfiniteList.head_drop]
+    simp only [ChaseDerivationSkeleton.next, cd2, derivation_for_skeleton, cds2, ChaseDerivationSkeleton.derivation_for_branch_suffix, PossiblyInfiniteList.tail_drop, PossiblyInfiniteList.head_drop]
     rw [Nat.succ_pred (Nat.ne_zero_of_lt lt)]
     exact eq_j
   apply (cd2.active_trigger_origin_next next_eq).right
   apply obs.contains_trg_result_implies_cond
   have sub : node.facts ⊆ cd2.head.facts := by
     let node : cd.Node := ⟨node, by exists i⟩
-    let node2 : cd.Node := ⟨cd2.head, by exists j.pred; simp only [cd2, derivation_for_branch_suffix, head, Option.some_get, PossiblyInfiniteList.head_drop]; rfl⟩
+    let node2 : cd.Node := ⟨cd2.head, by exists j.pred; simp only [cd2, derivation_for_skeleton, cds2, ChaseDerivationSkeleton.derivation_for_branch_suffix, ChaseDerivationSkeleton.head, Option.some_get, PossiblyInfiniteList.head_drop]; rfl⟩
     have prec : node ≼ node2 := by
       exists cd.derivation_for_branch_suffix (cd.branch.drop i) (PossiblyInfiniteList.IsSuffix_drop i) (by simp [PossiblyInfiniteList.head_drop, eq_i])
-      simp only [derivation_for_branch_suffix, head, PossiblyInfiniteList.head_drop]
+      simp only [ChaseDerivationSkeleton.derivation_for_branch_suffix, ChaseDerivationSkeleton.head, PossiblyInfiniteList.head_drop]
       constructor; exact PossiblyInfiniteList.IsSuffix_drop i
       constructor; simp [eq_i, node]
-      apply mem_of_mem_suffix (cd1 := cd2) _ _ cd2.head_mem
+      apply ChaseDerivationSkeleton.mem_of_mem_suffix (cd1 := cds2) _ _ cd2.head_mem
       exists j.pred - i
-      simp only [cd2, derivation_for_branch_suffix, PossiblyInfiniteList.drop]
+      simp only [cds2, ChaseDerivationSkeleton.derivation_for_branch_suffix, PossiblyInfiniteList.drop]
       apply InfiniteList.ext; intro n
       simp only [InfiniteList.get_drop, ← Nat.add_assoc, Nat.add_sub_of_le le]
     exact cd.facts_node_subset_of_prec prec
@@ -967,7 +699,8 @@ theorem prop_for_node_has_minimal_such_node {cd : ChaseDerivation obs rules} (pr
     intro le; simp only [Nat.not_lt] at le
     apply strict_predecessor_asymmetric prec
     constructor
-    . have n2_mem' : n2 ∈ cd := by exists k
+    . rw [predecessor_iff]
+      have n2_mem' : n2 ∈ cd := by exists k
       rcases cd.subderivation_of_node_mem n2_mem' with ⟨cd2, head2, suf2⟩
       exists cd2; simp only [suf2, head2, true_and]
       exists j - k
@@ -975,7 +708,7 @@ theorem prop_for_node_has_minimal_such_node {cd : ChaseDerivation obs rules} (pr
       have : k' = k := by
         apply cd.get?_branch_injective n2
         . rw [← head2]
-          simp only [head, Option.some_get, PossiblyInfiniteList.head]
+          simp only [ChaseDerivationSkeleton.head, Option.some_get, PossiblyInfiniteList.head]
           rw [← suf2]
           rfl
         . exact n2_mem
@@ -987,5 +720,4 @@ theorem prop_for_node_has_minimal_such_node {cd : ChaseDerivation obs rules} (pr
 end MinimalNodeWithProp
 
 end ChaseDerivation
-
 
